Add post invariants

managerOnlyUpdates - with changes.dfy
@@ -1,145 +1,161 @@
 function isPublisherOut (publisher : Publisher, ads: map <Publisher, Ad>, publishers : seq<Publisher>) : bool
-{
-	publisher !in publishers && publisher !in ads
-}
+        {
+        publisher !in publishers &&
+        publisher !in ads
+        }
 
-function arePublishersInBothLists (ads: map <Publisher, Ad>, publishers : seq<Publisher>) : bool
-{
-	(forall p :: p in publishers ==> p in ads) && (forall p :: p in ads ==> p in publishers)
-}
+        function adsKeysEqualsPublishers (ads: map <Publisher, Ad>, publishers : seq<Publisher>) : bool
+        {
+        (forall p :: p in publishers ==> p in ads) &&
+        (forall p :: p in ads ==> p in publishers)
+        }
 
-function valuesOfAds (myAds : map<Publisher, Ad>) : set<Ad>
+        function valuesOfAds (myAds : map<Publisher, Ad>) : set<Ad>
 {
-	set p: Publisher | p in myAds :: myAds[p]
-}
+        set p: Publisher | p in myAds :: myAds[p]
+        }
 
-function isNoNullPublishers (ads: map <Publisher, Ad>, publishers : seq<Publisher>) : bool
-requires arePublishersInBothLists(ads, publishers)
-reads valuesOfAds(ads)
-{
-	forall p :: p in publishers ==> p != null && ads[p] != null && ads[p].banner != null
-}
+        function isNoNullPublishers (ads: map <Publisher, Ad>, publishers : seq<Publisher>) : bool
+        requires adsKeysEqualsPublishers(ads, publishers)
+        reads valuesOfAds(ads)
+        {
+        forall p :: p in publishers ==> p != null && ads[p] != null && ads[p].banner != null
+        }
 
-function isNoNullAds (ads: map <Publisher, Ad>) : bool
-{
-	forall p :: p in ads ==> ads[p] != null
-}
+        function isNoNullAds (ads: map <Publisher, Ad>) : bool
+        {
+        forall p :: p in ads ==> ads[p] != null
+        }
 
-function isNoNullAvailableBanners (availableBanners: seq<Banner>) : bool
-{
-	forall i :: 0 <= i < |availableBanners| ==> availableBanners[i] != null
-}
+        function isNoNullAvailableBanners (availableBanners: seq<Banner>) : bool
+        {
+        forall i :: 0 <= i < |availableBanners| ==> availableBanners[i] != null
+        }
 
-function isUniqueAvailableBanners (availableBanners: seq<Banner>) : bool
-{
-	|availableBanners| > 0 ==> availableBanners[0] !in availableBanners[1..]
-}
+        function isUniqueAvailableBanners (availableBanners: seq<Banner>) : bool
+        {
+        |availableBanners| > 0 ==> availableBanners[0] !in availableBanners[1..]
+        }
 
-function isPublisherInMap (publisher : Publisher, retAds: map <Publisher, Ad>) : bool
-{
-	publisher in retAds && retAds[publisher] != null
-}
+        function isPublisherInMap (publisher : Publisher, retAds: map <Publisher, Ad>) : bool
+        {
+        publisher in retAds &&
+        retAds[publisher] != null
+        }
 
-function checkStartPublishRoomInAvailableBanners(publisher : Publisher, price : int, publishers : seq<Publisher>, retPublishers: seq<Publisher>, ads : map <Publisher, Ad>, retAds: map <Publisher, Ad>, availableBanners : seq<Banner>, retBanners: seq<Banner>) : bool
-reads valuesOfAds(retAds)
-{
-	|availableBanners| > 0 ==> publisher in retPublishers && publisher in retAds && retAds[publisher] != null && retAds[publisher].price == price  && availableBanners[0] == retAds[publisher].banner && retBanners == availableBanners[1..] && availableBanners[0] !in retBanners
-}
+        function checkStartPublishRoomInAvailableBanners(publisher : Publisher, price : int, publishers : seq<Publisher>, retPublishers: seq<Publisher>, ads : map <Publisher, Ad>, retAds: map <Publisher, Ad>, availableBanners : seq<Banner>, retBanners: seq<Banner>) : bool
+        reads valuesOfAds(retAds)
+        { //must add enters here - I don't know the scopes:
+        |availableBanners| > 0 ==> publisher in retPublishers && publisher in retAds && retAds[publisher] != null && retAds[publisher].price == price  && availableBanners[0] == retAds[publisher].banner && retBanners == availableBanners[1..] && availableBanners[0] !in retBanners
+        }
 
-function checkStartPublishAllListsEmpty (publisher : Publisher, price : int, publishers : seq<Publisher>, retPublishers: seq<Publisher>, ads : map <Publisher, Ad>, retAds: map <Publisher, Ad>, availableBanners : seq<Banner>, retBanners: seq<Banner>) : bool
-{
-	(|availableBanners| == 0 && |publishers| == 0) ==> publishers == retPublishers && ads == retAds && availableBanners == retBanners && publisher !in publishers && publisher !in ads
-}
+        function checkStartPublishAllListsEmpty (publisher : Publisher, price : int, publishers : seq<Publisher>, retPublishers: seq<Publisher>, ads : map <Publisher, Ad>, retAds: map <Publisher, Ad>, availableBanners : seq<Banner>, retBanners: seq<Banner>) : bool
+        {
+        (|availableBanners| == 0 && |publishers| == 0) ==> publishers == retPublishers && ads == retAds && availableBanners == retBanners && publisher !in publishers && publisher !in ads
+        }
 
-function checkStartPublishBidAccepted (publisher : Publisher, price : int, publishers : seq<Publisher>, retPublishers: seq<Publisher>, ads : map <Publisher, Ad>, retAds: map <Publisher, Ad>, availableBanners : seq<Banner>, retBanners: seq<Banner>, globalMinPublisher: Publisher) : bool
-reads valuesOfAds(retAds)
-reads valuesOfAds(ads)
-requires forall p :: p in ads ==> ads[p] != null
-{
-	(|availableBanners| == 0 && |publishers| > 0 && !isPriceLessThanMinPrice(price, ads)) ==> (publisher in retPublishers && isPublisherInMap(publisher, retAds) && retAds[publisher].price == price && availableBanners == retBanners) && (globalMinPublisher !in retPublishers && globalMinPublisher !in retAds && globalMinPublisher in ads && retAds[publisher].banner == ads[globalMinPublisher].banner)
-}
+        function checkStartPublishBidAccepted (publisher : Publisher, price : int, publishers : seq<Publisher>, retPublishers: seq<Publisher>, ads : map <Publisher, Ad>, retAds: map <Publisher, Ad>, availableBanners : seq<Banner>, retBanners: seq<Banner>, globalMinPublisher: Publisher) : bool
+        reads valuesOfAds(retAds)
+        reads valuesOfAds(ads)
+        requires forall p :: p in ads ==> ads[p] != null
+        {
+        (|availableBanners| == 0 && |publishers| > 0 && !isPriceLessThanMinPrice(price, ads)) ==> (publisher in retPublishers && isPublisherInMap(publisher, retAds) && retAds[publisher].price == price && availableBanners == retBanners) && (globalMinPublisher !in retPublishers && globalMinPublisher !in retAds && globalMinPublisher in ads && retAds[publisher].banner == ads[globalMinPublisher].banner)
+        }
 
-function isPriceLessThanMinPrice (price : int, ads: map <Publisher, Ad>) : bool
-reads valuesOfAds(ads)
-//requires forall p :: p in ads ==> ads[p] != null
-{
-	forall p :: p in ads && ads[p] != null ==> ads[p].price >= price
-}
+        function isPriceLessThanMinPrice (price : int, ads: map <Publisher, Ad>) : bool
+        reads valuesOfAds(ads)
+        {
+        forall p :: p in ads && ads[p] != null ==> ads[p].price >= price
+        }
 
-function checkStartPublishBidNotAccepted (publisher : Publisher, price : int, publishers : seq<Publisher>, retPublishers: seq<Publisher>, ads : map <Publisher, Ad>, retAds: map <Publisher, Ad>, availableBanners : seq<Banner>, retBanners: seq<Banner>) : bool
-reads valuesOfAds(ads)
-{
-	(|availableBanners| == 0 && |publishers| > 0 && isPriceLessThanMinPrice(price, ads)) ==> publishers == retPublishers && ads == retAds && availableBanners == retBanners && isPublisherOut(publisher, ads, publishers)
-}
+        function checkStartPublishBidNotAccepted (publisher : Publisher, price : int, publishers : seq<Publisher>, retPublishers: seq<Publisher>, ads : map <Publisher, Ad>, retAds: map <Publisher, Ad>, availableBanners : seq<Banner>, retBanners: seq<Banner>) : bool
+        reads valuesOfAds(ads)
+        {
+        (|availableBanners| == 0 && |publishers| > 0 && isPriceLessThanMinPrice(price, ads)) ==> publishers == retPublishers && ads == retAds && availableBanners == retBanners && isPublisherOut(publisher, ads, publishers)
+        }
 
-function isNoNull (availableBanners: seq<Banner>, publishers : seq<Publisher>, ads : map <Publisher, Ad>)  : bool
-reads valuesOfAds(ads)
-requires arePublishersInBothLists(ads, publishers)
-{
-	isNoNullPublishers(ads,publishers) && isNoNullAds(ads) && isNoNullAvailableBanners(availableBanners)
-}
+        function isNoNull (availableBanners: seq<Banner>, publishers : seq<Publisher>, ads : map <Publisher, Ad>)  : bool
+        reads valuesOfAds(ads)
+        requires adsKeysEqualsPublishers(ads, publishers)
+        {
+        isNoNullPublishers(ads,publishers) && isNoNullAds(ads) && isNoNullAvailableBanners(availableBanners)
+        }
 
-function adExists(adService : AdvertisingService, publisher: Publisher, ads: map <Publisher, Ad>, availableBanners: seq<Banner>) : bool
-reads valuesOfAds(ads)
-{
-	adService != null  && isPublisherInMap(publisher, ads) && ads[publisher].banner !in availableBanners 
-}
+        function adExists(adService : AdvertisingService, publisher: Publisher, ads: map <Publisher, Ad>, availableBanners: seq<Banner>) : bool
+        reads valuesOfAds(ads)
+        {
+        isPublisherInMap(publisher, ads) && ads[publisher].banner !in availableBanners
+        }
 
-function startPublishCorrectChanges (publisher: Publisher, availableBanners: seq<Banner>, publishers : seq<Publisher>, ads : map <Publisher, Ad>)  : bool
-reads valuesOfAds(ads)
-{
-	isPublisherOut(publisher, ads, publishers) && arePublishersInBothLists(ads, publishers) && isUniqueAvailableBanners(availableBanners) 
-}
+        function startPublishRequirements (publisher: Publisher, availableBanners: seq<Banner>, publishers : seq<Publisher>, ads : map <Publisher, Ad>)  : bool
+        reads valuesOfAds(ads)
+        {
+        isPublisherOut(publisher, ads, publishers) && adsKeysEqualsPublishers(ads, publishers) && isUniqueAvailableBanners(availableBanners) && adsKeysEqualsPublishers(ads, publishers)
+        }
 
-function findMinPublisherPreConditions(publishers : seq<Publisher>, ads : map <Publisher, Ad>) : bool 
-reads valuesOfAds(ads)
-{
-	|publishers| > 0 && forall p :: p in publishers ==> p != null && p in ads && ads[p] != null && ads[p].banner != null && arePublishersInBothLists(ads, publishers) && isNoNullAds(ads)
-}
+        function findMinPublisherPreConditions(publishers : seq<Publisher>, ads : map <Publisher, Ad>) : bool
+        reads valuesOfAds(ads)
+        {
+        |publishers| > 0 && forall p :: p in publishers ==> p != null && p in ads && ads[p] != null && ads[p].banner != null && adsKeysEqualsPublishers(ads, publishers) && isNoNullAds(ads)
+        }
 
-function findMinPublisherPostConditions(retPrice : int, retPublisher : Publisher, publishers : seq<Publisher>, ads : map <Publisher, Ad>) : bool 
-requires forall p :: p in ads ==> ads[p] != null
-reads valuesOfAds(ads)
-{
-	retPublisher in ads && retPublisher in publishers && retPublisher != null && ads[retPublisher] != null && ads[retPublisher].banner != null && ads[retPublisher].price == retPrice && forall p :: p in ads ==> ads[p].price >= retPrice
-}
+        function findMinPublisherPostConditions(retPrice : int, retPublisher : Publisher, publishers : seq<Publisher>, ads : map <Publisher, Ad>) : bool
+        requires forall p :: p in ads ==> ads[p] != null
+        reads valuesOfAds(ads)
+        {
+        retPublisher in ads && retPublisher in publishers && retPublisher != null && ads[retPublisher] != null && ads[retPublisher].banner != null && ads[retPublisher].price == retPrice && forall p :: p in ads ==> ads[p].price >= retPrice
+        }
 
-function startPublishPostConditions(publisher : Publisher, price : int, publishers : seq<Publisher>, retPublishers: seq<Publisher>, ads : map <Publisher, Ad>, retAds: map <Publisher, Ad>, availableBanners : seq<Banner>, retBanners: seq<Banner>, globalMinPublisher: Publisher) : bool
-reads valuesOfAds(retAds)
-reads valuesOfAds(ads)
-requires forall p :: p in ads ==> ads[p] != null
-{
-	checkStartPublishRoomInAvailableBanners(publisher, price, publishers, retPublishers, ads, retAds, availableBanners, retBanners)
-	&& checkStartPublishBidNotAccepted(publisher, price, publishers, retPublishers, ads, retAds, availableBanners, retBanners)
-	&& checkStartPublishBidAccepted(publisher, price, publishers, retPublishers, ads, retAds, availableBanners, retBanners, globalMinPublisher)
-	&& checkStartPublishAllListsEmpty(publisher, price, publishers, retPublishers, ads, retAds, availableBanners, retBanners)
-}
+        function startPublishPostConditions(publisher : Publisher, price : int, publishers : seq<Publisher>, retPublishers: seq<Publisher>, ads : map <Publisher, Ad>, retAds: map <Publisher, Ad>, availableBanners : seq<Banner>, retBanners: seq<Banner>, globalMinPublisher: Publisher) : bool
+        reads valuesOfAds(retAds)
+        reads valuesOfAds(ads)
+        requires forall p :: p in ads ==> ads[p] != null
+        {
+        checkStartPublishRoomInAvailableBanners(publisher, price, publishers, retPublishers, ads, retAds, availableBanners, retBanners)
+        && checkStartPublishBidNotAccepted(publisher, price, publishers, retPublishers, ads, retAds, availableBanners, retBanners)
+        && checkStartPublishBidAccepted(publisher, price, publishers, retPublishers, ads, retAds, availableBanners, retBanners, globalMinPublisher)
+        && checkStartPublishAllListsEmpty(publisher, price, publishers, retPublishers, ads, retAds, availableBanners, retBanners)
+        }
 
-function removePublisherInvPublisherOut(index: int, publishers: seq<Publisher>, newPublishers: seq<Publisher>, publisher: Publisher) : bool
-{
-	0 <= index <= |publishers| && publisher !in newPublishers
-}
+        function removePublisherInvPublisherOut(index: int, publishers: seq<Publisher>, newPublishers: seq<Publisher>, publisher: Publisher) : bool
+        {
+        0 <= index <= |publishers| && publisher !in newPublishers
+        }
 
-function removePublisherInvRestIn(index: int, publishers: seq<Publisher>, newPublishers: seq<Publisher>, publisher: Publisher) : bool
-requires index <= |publishers|
-{
-	forall i :: 0 <= i < index && publishers[i] != publisher ==> publishers[i] in newPublishers
-}
+        function removePublisherInvRestIn(index: int, publishers: seq<Publisher>, newPublishers: seq<Publisher>, publisher: Publisher) : bool
+        requires index <= |publishers|
+        {
+        forall i :: 0 <= i < index && publishers[i] != publisher ==> publishers[i] in newPublishers
+        }
 
 
-function findMinPublisherInvDataStructuresOk(minPrice: int, ads : map <Publisher, Ad>, index: int, publishers: seq<Publisher>, minPublisher: Publisher) : bool
-reads valuesOfAds(ads)
-{
-	forall p :: p in publishers ==> p in ads && minPublisher in ads && ads[minPublisher] != null && ads[minPublisher].price == minPrice && minPublisher in publishers
-}
+        function findMinPublisherInvDataStructuresOk(minPrice: int, ads : map <Publisher, Ad>, index: int, publishers: seq<Publisher>, minPublisher: Publisher) : bool
+        reads valuesOfAds(ads)
+        {
+        forall p :: p in publishers ==> p in ads && minPublisher in ads && ads[minPublisher] != null && ads[minPublisher].price == minPrice && minPublisher in publishers
+        }
 
-function findMinPublisherInvMinPriceCorrect(minPrice: int, ads : map <Publisher, Ad>, index: int, publishers: seq<Publisher>, minPublisher: Publisher) : bool
-requires isNoNullAds(ads)
-requires arePublishersInBothLists(ads, publishers)
-reads valuesOfAds(ads)
-{
-	0 <= index <= |publishers| && minPublisher in ads && forall i :: 0 <= i < index ==> minPrice <= ads[publishers[i]].price && isNoNullAds(ads)
-}
+        function findMinPublisherInvMinPriceCorrect(minPrice: int, ads : map <Publisher, Ad>, index: int, publishers: seq<Publisher>, minPublisher: Publisher) : bool
+        requires isNoNullAds(ads)
+        requires adsKeysEqualsPublishers(ads, publishers)
+        reads valuesOfAds(ads)
+        {
+        0 <= index <= |publishers| && minPublisher in ads && forall i :: 0 <= i < index ==> minPrice <= ads[publishers[i]].price && isNoNullAds(ads)
+        }
+
+
+        function bannerRemovedInvariant(banner : Banner, retBanners : seq<Banner>, availableBanners : seq<Banner>) : bool
+        {
+        banner !in retBanners &&
+        forall b :: b in availableBanners && b != banner ==> b in retBanners
+        }
+
+        function adRemovedInvariant(publisher : Publisher, retAds : map <Publisher, Ad>, ads : map <Publisher, Ad>) : bool
+        {
+        publisher !in retAds &&
+        forall p :: p in ads && p != publisher ==> p in retAds && retAds[p] == ads[p]
+        }
+
 
 class AdvertisingManager {
 
@@ -162,84 +178,58 @@ class AdvertisingManager {
 
     method addBanner(banner : Banner)
     modifies this
-    requires adService != null
-    requires banner !in availableBanners
-    //ensures banner in availableBanners
+    requires adService != null && banner !in availableBanners
     {
         availableBanners := adService.addBanner(banner, availableBanners);
     }
 
-	method removeBanner(banner : Banner)
+    method removeBanner(banner : Banner)
     modifies this
-    requires adService != null
-    requires banner in availableBanners
+    requires adService != null && banner in availableBanners
     {
         availableBanners := adService.removeBanner(banner, availableBanners);
     }
-    
-    /*    
-    method stopPublish (publisher: Publisher) //wrapper method for stopPublishAndFreeBanner (just to keep pointer for banner in the post-condition)
+
+    method stopPublish (publisher: Publisher)
     modifies this
-    requires adService != null
-    requires publisher in ads && ads[publisher] != null
-    requires ads[publisher].banner !in availableBanners 
-	ensures publisher !in publishers
-    ensures publisher !in ads
+    requires adExists(adService, publisher, ads, availableBanners) && adService != null
     {
-      stopPublish(publisher, ads[publisher].banner);
+        publishers := adService.removePublisher(publisher, publishers);
+        availableBanners := adService.addBanner(ads[publisher].banner, availableBanners);
+        ads := adService.removeAdOfPublisher(publisher, ads);
     }
-    */
-    
-    method stopPublish (publisher: Publisher) 
-    modifies this
-	requires adExists(adService, publisher, ads, availableBanners)
-    //requires banner !in availableBanners    
-    //ensures publisher !in publishers
-    //ensures publisher !in ads
-    //ensures banner in availableBanners
-    {
-      publishers := adService.removePublisher(publisher, publishers);
-      availableBanners := adService.addBanner(ads[publisher].banner, availableBanners);
-      ads := adService.removeAdOfPublisher(publisher, ads);      
-    }
-    
-    method startPublish (publisher : Publisher, price : int) 
+
+    method startPublish (publisher : Publisher, price : int)
     modifies this
     modifies adService
-	requires arePublishersInBothLists(ads, publishers)
-	requires isNoNull (availableBanners, publishers, ads) &&  adService != null
-	requires startPublishCorrectChanges(publisher, availableBanners, publishers, ads)
+    requires startPublishRequirements(publisher, availableBanners, publishers, ads)
+    requires isNoNull (availableBanners, publishers, ads) &&  adService != null
     {
         publishers, ads, availableBanners := adService.startPublish(publisher, price, publishers, ads, availableBanners);
     }
-	
-	method isInPublishers(publisher : Publisher) returns (status : bool)
-	requires arePublishersInBothLists (ads, publishers)
-	ensures publisher in publishers <==> status == true
-	{
-		return publisher in publishers;
-	} 
-	
-	method isBannerAvailable(banner : Banner) returns (status : bool)
-	ensures banner in availableBanners <==> status == true
-	{
-		return banner in availableBanners;
-	}         
+
+    method isPublishing(publisher : Publisher) returns (status : bool)
+    requires adsKeysEqualsPublishers (ads, publishers)
+    ensures publisher in publishers <==> status == true
+    {
+        return publisher in publishers;
+    }
+
+    method isBannerAvailable(banner : Banner) returns (status : bool)
+    ensures banner in availableBanners <==> status == true
+    {
+        return banner in availableBanners;
+    }
 }
 
-class AdvertisingService 
+class AdvertisingService
 {
     var globalMinPublisher: Publisher;
 
-    constructor () 
-    {  
+    constructor ()
+    {
     }
 
-	//function isInside (b: Banner, s: seq<Banner>) : bool
-    //{
-      //b in s
-    //}
-    
     method addBanner(banner : Banner, banners : seq<Banner>) returns (retBanners : seq<Banner>)
     requires banner !in banners
     ensures banner in retBanners
@@ -247,17 +237,16 @@ class AdvertisingService
         return banners + [banner];
     }
 
-	method removeBanner(banner : Banner, availableBanners : seq<Banner>) returns (retBanners : seq<Banner>)
+    method removeBanner(banner : Banner, availableBanners : seq<Banner>) returns (retBanners : seq<Banner>)
     requires banner in availableBanners
-    ensures banner !in retBanners
-	ensures forall b :: b in availableBanners && b != banner ==> b in retBanners
+    ensures bannerRemovedInvariant (banner, retBanners, availableBanners)
     {
-		var index := 0;
-		var newBanners : seq<Banner> := [];
+        var index := 0;
+        var newBanners : seq<Banner> := [];
         while (index < |availableBanners|)
-        decreases |availableBanners| - index // not needed - but it seems more complicated :)
+            decreases |availableBanners| - index
         invariant 0 <= index <= |availableBanners| && banner !in newBanners
-		invariant forall i :: 0 <= i < index && availableBanners[i] != banner ==> availableBanners[i] in newBanners 
+        invariant forall i :: 0 <= i < index && availableBanners[i] != banner ==> availableBanners[i] in newBanners
         {
             if (availableBanners[index] != banner)
             {
@@ -267,14 +256,13 @@ class AdvertisingService
         }
         return newBanners;
     }
-    
+
     method removeAdOfPublisher(publisher : Publisher, ads : map <Publisher, Ad>) returns (retAds : map <Publisher, Ad>)
-    ensures publisher !in retAds
-    ensures forall p :: p in ads && p != publisher ==> p in retAds && retAds[p] == ads[p]
+    ensures adRemovedInvariant(publisher, retAds, ads)
     {
-      return map p | p in ads && p != publisher :: ads[p];
+        return map p | p in ads && p != publisher :: ads[p];
     }
-    
+
     method removePublisher(publisher : Publisher, publishers : seq<Publisher>) returns (retPublishers : seq<Publisher>)
     ensures publisher !in retPublishers
     ensures forall p :: p in publishers && p != publisher ==> p in retPublishers
@@ -282,7 +270,7 @@ class AdvertisingService
         var index := 0;
         var newPublishers : seq<Publisher> := [];
         while (index < |publishers|)
-        decreases |publishers| - index // not needed - but it seems more complicated :)
+            decreases |publishers| - index
         invariant removePublisherInvPublisherOut(index, publishers, newPublishers, publisher)
         invariant removePublisherInvRestIn(index, publishers, newPublishers, publisher)
         {
@@ -295,141 +283,107 @@ class AdvertisingService
 
         return newPublishers;
     }
-    
+
     method addPublisher (publisher : Publisher, publishers : seq<Publisher>) returns (retPublishers : seq<Publisher>)
     ensures publisher in retPublishers
-	ensures forall p :: p in publishers ==> p in retPublishers
+    ensures forall p :: p in publishers ==> p in retPublishers
     {
-      return publishers + [publisher];     
+        return publishers + [publisher];
     }
-    
+
     method addAd (publisher : Publisher, price : int, banner : Banner, ads : map <Publisher, Ad>) returns (retAds : map <Publisher, Ad>)
-    requires banner != null; 
+    requires banner != null;
     ensures isPublisherInMap(publisher, retAds)
     ensures retAds[publisher].price == price && retAds[publisher].banner == banner
     {
-      var newAd : Ad := new Ad(banner, price);
-      return ads[publisher := newAd]; 
+        var newAd : Ad := new Ad(banner, price);
+        return ads[publisher := newAd];
     }
-    
+
     method popFirstBanner(banners : seq<Banner>) returns (retBanners : seq<Banner>)
     requires |banners| > 0
-    requires banners[0] !in banners[1..] //- need to ensures it in a more general way ==> I THINK ITS OK NOW 
-    ensures banners[0] !in retBanners    // - need to ensures it in a more general way ==> I THINK ITS OK NOW 
-	ensures retBanners == banners[1..]
+    requires banners[0] !in banners[1..]
+    ensures banners[0] !in retBanners
+    ensures retBanners == banners[1..]
     {
-      return banners[1..];
+        return banners[1..];
     }
 
-	//function checkInvariantFindMinPublisher(index: int, publishers : seq<Publisher>, ads : map <Publisher, Ad>, minPublisher: Publisher, minPrice: int): bool
-	//{
-		//(forall p :: p in publishers ==> p in ads && minPublisher in ads && ads[minPublisher] != null && ads[minPublisher].price == minPrice && minPublisher in publishers) && (0 <= index <= |publishers| && minPublisher in ads && forall i :: 0 <= i < index ==> minPrice <= ads[publishers[i]].price && forall p :: p in ads ==> ads[p] != null)
-	//}  
-    
-    // WE CAN NOW CHANGE THIS METHOD TO USE THE NEW FUNCTIONS - BUT IT MAY CHANGE THE CONDITIONS :( 
     method findMinPublisher(publishers : seq<Publisher>, ads : map <Publisher, Ad>) returns (retPublisher : Publisher, retPrice : int)
-	requires findMinPublisherPreConditions(publishers, ads)
-	requires forall p :: p in ads ==> ads[p] != null
-	ensures findMinPublisherPostConditions(retPrice, retPublisher, publishers, ads)
-    {
-      var minPublisher := publishers[0];
-      var minPrice := ads[minPublisher].price;
-
-      var index := 1;
-      while (index < |publishers|)
-      decreases |publishers| - index
-	  invariant findMinPublisherInvDataStructuresOk(minPrice, ads, index, publishers, minPublisher)
-	  invariant findMinPublisherInvMinPriceCorrect(minPrice, ads, index, publishers, minPublisher)
-	  // checkInvariantFindMinPublisher(index, publishers, ads,minPublisher, minPrice);
-	  {
-        var curPrice := ads[publishers[index]].price;
-        if (curPrice < minPrice)
-        {
-          minPrice := curPrice;
-          minPublisher := publishers[index];
-        }
-        index := index + 1;
-      }
-      return minPublisher, minPrice;
-    }    
-    
-
-/*
-    // need to add ensures...     
-    function minPublisherFunc (publishers : seq<Publisher>, ads : map<Publisher, Ad>, tempMin : Publisher) : Publisher
-    reads valuesOfAds(ads)
-    requires forall p :: p in publishers ==> p in ads && ads[p] != null
+    requires findMinPublisherPreConditions(publishers, ads)
     requires forall p :: p in ads ==> ads[p] != null
-    requires tempMin in ads && ads[tempMin] != null
-    ensures minPublisherFunc(publishers, ads, tempMin) in ads && ads[minPublisherFunc(publishers, ads, tempMin)] != null
-    ensures forall p :: p in publishers ==> ads[p].price >= ads[minPublisherFunc(publishers, ads, tempMin)].price
+    ensures findMinPublisherPostConditions(retPrice, retPublisher, publishers, ads)
     {
-      if publishers == [] then tempMin else minPublisherFunc(publishers[1..], ads, minFunc(tempMin, publishers[0], ads))
+        var minPublisher := publishers[0];
+        var minPrice := ads[minPublisher].price;
+
+        var index := 1;
+        while (index < |publishers|)
+            decreases |publishers| - index
+        invariant findMinPublisherInvDataStructuresOk(minPrice, ads, index, publishers, minPublisher)
+        invariant findMinPublisherInvMinPriceCorrect(minPrice, ads, index, publishers, minPublisher)
+        // checkInvariantFindMinPublisher(index, publishers, ads,minPublisher, minPrice);
+        {
+            var curPrice := ads[publishers[index]].price;
+            if (curPrice < minPrice)
+            {
+                minPrice := curPrice;
+                minPublisher := publishers[index];
+            }
+            index := index + 1;
+        }
+        return minPublisher, minPrice;
     }
-    
-    function minFunc (p1 : Publisher, p2 : Publisher, ads : map<Publisher, Ad>) : Publisher
-    reads valuesOfAds(ads)
-    requires p1 in ads && p2 in ads && ads[p1] != null && ads[p2] != null
-    {
-      if ads[p1].price <= ads[p2].price then p1 else p2
-    }
-    */
-    
-
-
-
-
 
     method startPublish(publisher : Publisher, price : int, publishers : seq<Publisher>, ads : map <Publisher, Ad>, availableBanners : seq<Banner>) returns (retPublishers : seq<Publisher>, retAds : map <Publisher, Ad>, retBanners : seq<Banner>)
     modifies this
-	
-	requires startPublishCorrectChanges(publisher, availableBanners, publishers, ads)
-	requires isNoNull (availableBanners, publishers, ads) 
-	ensures startPublishPostConditions(publisher, price, publishers, retPublishers, ads, retAds, availableBanners, retBanners, globalMinPublisher);
+    requires startPublishRequirements(publisher, availableBanners, publishers, ads)
+    requires isNoNull (availableBanners, publishers, ads)
+    ensures startPublishPostConditions(publisher, price, publishers, retPublishers, ads, retAds, availableBanners, retBanners, globalMinPublisher);
 
-	{
-      var newPublishers : seq<Publisher> := publishers;
-      var newAds : map <Publisher, Ad> := ads;
-      var newBanners : seq<Banner> := availableBanners;
-      
-      if (|availableBanners| > 0)
-      {
-        newPublishers := addPublisher(publisher, newPublishers);
-        newAds := addAd(publisher, price, newBanners[0], newAds);          
-        newBanners := popFirstBanner(newBanners);               
-      } 
-      else
-      {
-        if (|newPublishers| > 0)
+    {
+        var newPublishers : seq<Publisher> := publishers;
+        var newAds : map <Publisher, Ad> := ads;
+        var newBanners : seq<Banner> := availableBanners;
+
+        if (|availableBanners| > 0)
         {
-          var minPublisher, minPrice := findMinPublisher(newPublishers, newAds);
-          globalMinPublisher := minPublisher;
-          if (price > minPrice) 
-          {
-            var banner := newAds[minPublisher].banner;
-            newAds := addAd(publisher, price, banner, newAds);
-            newAds := removeAdOfPublisher(minPublisher, newAds);   
-            newPublishers := addPublisher(publisher, newPublishers); 
-            newPublishers := removePublisher(minPublisher, newPublishers);   
-          }
+            newPublishers := addPublisher(publisher, newPublishers);
+            newAds := addAd(publisher, price, newBanners[0], newAds);
+            newBanners := popFirstBanner(newBanners);
         }
-      }  
-      
-     return newPublishers, newAds, newBanners; 
-    }        
-        
+      else
+        {
+            if (|newPublishers| > 0)
+            {
+                var minPublisher, minPrice := findMinPublisher(newPublishers, newAds);
+                globalMinPublisher := minPublisher;
+                if (price > minPrice)
+                {
+                    var banner := newAds[minPublisher].banner;
+                    newAds := addAd(publisher, price, banner, newAds);
+                    newAds := removeAdOfPublisher(minPublisher, newAds);
+                    newPublishers := addPublisher(publisher, newPublishers);
+                    newPublishers := removePublisher(minPublisher, newPublishers);
+                }
+            }
+        }
+
+        return newPublishers, newAds, newBanners;
+    }
+
 }
 
 class Publisher
 {
-    constructor () 
+    constructor ()
     {
     }
 }
 
 class Banner
 {
-    constructor () 
+    constructor ()
     {
     }
 }
@@ -448,21 +402,6 @@ class Ad
         banner := bannerArg;
         price := priceArg;
     }
-    
-    /* THESE GETTERS ONLY CAUSE PROBLEMS 
-
-    method getBanner() returns (b: Banner)
-    ensures b == banner;
-    {
-        return banner;
-    }
-
-    method getPrice() returns (p: int)
-    ensures p == price;
-    {
-        return price;
-    }
-    */
 }
 
 
